src/ordered_lemmas.lean
@@ -2,131 +2,24 @@ import btree
 set_option pp.generalized_field_notation false
 
 namespace ordered_lemmas
-open btree_def 
+open btree_def
 
-lemma ordered_insert {α : Type} (p : nat → btree α → Prop) (t : btree α) (k : nat) (a : α) :
-  ordered p t → p k t → ordered p (insert k a t) :=
+lemma ordered_insert {α : Type} (t : btree α) (k : nat) (a : α) :
+  ordered t → ordered (insert k a t) :=
 begin
-  intros h₁ h₂,
-  induction t,
-  case empty {
-    simp only [btree_def.insert, ordered],
-    apply and.intro,
-    { simp },
-    { apply and.intro, 
-      simp, apply and.intro, apply h₂, exact h₂},
-  },
-  case node : tl tk ta tr ihl ihr {
-    simp only [btree_def.insert],
-    by_cases c₁ : (k < tk),
-    { simp only [if_pos c₁, ordered],
-      apply and.intro, 
-      { apply ihl, 
-        { simp [ordered] at h₁, apply and.elim h₁,
-          intros h h', exact h, }, 
-        { sorry }, 
-      },
-      { apply and.intro, 
-        { simp [ordered] at h₁, apply and.elim h₁,
-          intros h h', apply and.elim h',
-          intros h₁ h₂, exact h₁, },
-        { apply and.intro, 
-          { sorry },
-          { simp [ordered] at h₁, apply and.elim h₁,
-            intros h h', apply and.elim h',
-            intros h₃ h₄, apply and.elim h₄, 
-            intros h₅ h₆, exact h₆, }, 
-        },
-      },
-    },
-    { simp only [if_neg c₁],
-      by_cases c₂ : (k > tk),
-      { simp only [if_pos c₂, ordered],
-        apply and.intro, 
-        { simp only [ordered] at h₁,
-          apply and.elim h₁,
-          intros h h', exact h, },
-        { simp only [ordered] at h₁,
-          apply and.intro,
-          { apply ihr,
-            { apply and.elim h₁,
-              intros h h',
-              apply and.elim h',
-              intros h₃ h₄, exact h₃,
-            },
-            { sorry },
-          },
-          { apply and.intro,
-            { apply and.elim h₁,
-              intros h h',
-              apply and.elim h',
-              intros h₃ h₄,
-              apply and.elim h₄,
-              intros h₅ h₆, exact h₅, },
-            { sorry },
-          }, 
-        }, 
-      },
-      { simp only [if_neg c₂, ordered],
-        apply and.intro,
-        { simp only [ordered] at h₁,
-          apply and.elim h₁,
-          intros h h', exact h, },
-        { apply and.intro, 
-          { simp only [ordered] at h₁,
-            apply and.elim h₁, 
-            intros h h', 
-            apply and.elim h',
-            intros h₂ h₃, exact h₂, 
-          }, 
-          { apply and.intro,
-            { sorry },
-            { sorry },
-          }, 
-        },
-      }, 
-    },
-  },
+  sorry
 end
 
-lemma ordered_lookup {α : Type} (p : nat → btree α → Prop) (s : btree α) (k : nat) (v : α) :
-  (ordered p s ∧ (bound k s)) → ((lookup k s) = some v) :=
-begin
-  intro h₁,
-  induction s,
-  case empty {
-    simp only [lookup], 
-    sorry,
-  },
-  case node : sl sk sa sr ihl ihr {
-    simp only [lookup],
-    by_cases h₂ : (k < sk),
-    { simp only [if_pos h₂], apply ihl, 
-      simp [ordered] at h₁, 
-      sorry, 
-    },
-    { simp only [if_neg h₂],
-      by_cases h₃ : (k > sk),
-      { simp [if_pos h₃],
-        apply ihr, sorry },
-      { simp [if_neg h₃], sorry } }
-  }
+lemma ordered_lookup {α : Type} (t : btree α) (k : nat) (a : α) :
+  ordered t ∧ bound k t → (lookup k t = some a) :=
+begin 
+  sorry
 end
 
-lemma unique_keys_nb {α : Type} (p : nat → btree α → Prop) (s : btree α) (k : nat) :
-  (ordered p s ∧ ((bound k s) = ff)) → ((treeElems s k ) = []) :=
+lemma unique_keys_nb {α : Type} (t : btree α) (k : nat) :
+  ordered t ∧ bound k t = ff → treeElems t k = [] :=
 begin
-  intro h₁,
-  induction s,
-  case empty {
-    refl,
-  },
-  case node : sl sk sa sr ihl ihr {
-    simp only [treeElems],
-    by_cases c₁ : (k = sk),
-    { simp only [if_pos c₁], sorry },
-    { simp only [if_neg c₁], sorry },
-  }
+  sorry
 end
 
 end ordered_lemmas
